wip: transpose

code/chacha20/Hacl.Spec.Chacha20.Lemmas.fst
@@ -6,6 +6,7 @@ open Lib.Sequence
 open Lib.IntVector
 
 open Hacl.Spec.Chacha20.Vec
+module Loop = Lib.LoopCombinators
 
 
 #set-options "--z3rlimit 50 --max_fuel 0 --max_ifuel 0"
@@ -17,22 +18,243 @@ unfold
 let op_Array_Access (#w:lanes) (a:uint32xN w) i = (vec_v a).[i]
 
 
+val transposewxf_f_lemma:
+    #w:lanes -> n:nat{pow2 n == w} -> i:nat{i < n} -> vs:lseq (uint32xN w) w
+  -> j:nat{j < pow2 i} -> k:nat{k < w / (2 * pow2 i)} ->
+  Lemma (let m2 = pow2 i in let m = 2 * m2 in let vs_kj = vs.[k * m + j] in
+    Math.Lemmas.pow2_multiplication_modulo_lemma_1 1 i n;
+    (transposewxw_f #w n i vs).[k * m + j] == vec_interleave_low_n m2 vs_kj vs.[k * m + j + m2] /\
+    (transposewxw_f #w n i vs).[k * m + j + m2] == vec_interleave_high_n m2 vs_kj vs.[k * m + j + m2])
+
+let transposewxf_f_lemma #w n i vs j k = admit()
+
+// val lemma_aux: #w:pos -> n:nat{pow2 n == w} -> i:nat{i < n} -> l:nat{l < w} -> Lemma
+//   (let m2 = pow2 i in let m = 2 * m2 in
+//    let k = l / m in let j = l % m in
+//    let j' = if j > m2 then j - m2 else j in
+//    l == (if j > m2 then k * m + j' + m2 else k * m + j'))
+// let lemma_aux #w n i l = ()
+
+val lemma_k_lt_wm: #w:pos -> n:nat{pow2 n == w} -> i:nat{i < n} -> l:nat{l < w} -> Lemma
+  (let m2 = pow2 i in let m = 2 * m2 in l / m < w / m)
+let lemma_k_lt_wm #w n i l =
+  let m2 = pow2 i in let m = 2 * m2 in
+  Math.Lemmas.pow2_plus 1 i;
+  assert (m == pow2 (i + 1));
+  let k = l / m in
+  assert (l < pow2 n);
+  Math.Lemmas.lemma_div_lt_nat l n (i + 1);
+  assert (l / m < pow2 (n - i - 1));
+  Math.Lemmas.pow2_minus n (i + 1);
+  assert (k < w / m)
+
+
+val lemma_l_plus_m2_lt: #w:pos -> n:nat{pow2 n == w} -> i:nat{i < n} -> l:nat{l < w} -> Lemma
+  (requires l % (2 * pow2 i) < pow2 i)
+  (ensures  (let m2 = pow2 i in let m = 2 * m2 in l / m * m + l % m + pow2 i < pow2 n))
+let lemma_l_plus_m2_lt #w n i l =
+  let m2 = pow2 i in let m = 2 * m2 in
+  let k = l / m in let j = l % m in
+  lemma_k_lt_wm #w n i l;
+  assert (k < w / m);
+  assert (j < m2);
+  assert (k * m + j + m2 < k * m + m);
+  assert (k * m + j + m2 < (k + 1) * m);
+  assert ((k + 1) * m <= w / m * m);
+  assert (k * m + j + m2 < w / m * m)
+
+
+val transposewxw_f_lemma_l:
+  #w:lanes -> n:nat{pow2 n == w} -> i:nat{i < n} -> vs:lseq (uint32xN w) w -> l:nat{l < w} -> Lemma
+  (if l % (2 * pow2 i) < pow2 i then begin
+    lemma_l_plus_m2_lt #w n i l;
+    Math.Lemmas.pow2_multiplication_modulo_lemma_1 1 i n;
+    (transposewxw_f #w n i vs).[l] == vec_interleave_low_n (pow2 i) vs.[l] vs.[l + pow2 i] end
+   else begin
+    Math.Lemmas.pow2_multiplication_modulo_lemma_1 1 i n;
+    (transposewxw_f #w n i vs).[l] == vec_interleave_high_n (pow2 i) vs.[l - pow2 i] vs.[l] end)
+
+let transposewxw_f_lemma_l #w n i vs l =
+  let m2 = pow2 i in
+  let m = 2 * m2 in
+  let k = l / m in
+  if l % (2 * pow2 i) < pow2 i then begin
+    let j = l % m in
+    lemma_k_lt_wm #w n i l;
+    transposewxf_f_lemma #w n i vs j k end
+  else begin
+    let j = l % m - m2 in
+    lemma_k_lt_wm #w n i l;
+    transposewxf_f_lemma #w n i vs j k end
+
+
 val transpose4x4_lemma_ij: vs:lseq (uint32xN 4) 4 -> i:nat{i < 4} -> j:nat{j < 4} ->
   Lemma ((vec_v (transpose4x4 vs).[i]).[j] == (vec_v vs.[j]).[i])
 let transpose4x4_lemma_ij vs i j =
-  admit()
+  let res = transposewxw 2 vs in
+  Loop.unfold_repeati 2 (transposewxw_f 2) vs 1;
+  Loop.unfold_repeati 2 (transposewxw_f 2) vs 0;
+  Loop.eq_repeati0 2 (transposewxw_f 2) vs;
+
+  let res0 = transposewxw_f 2 0 vs in
+  let res1 = transposewxw_f 2 1 res0 in
+  Classical.forall_intro (transposewxw_f_lemma_l #4 2 1 res0);
+  Classical.forall_intro (transposewxw_f_lemma_l #4 2 0 vs);
+
+  vec_interleave_low_n_lemma_uint32_4_2 res0.[0] res0.[2];
+  vec_interleave_high_n_lemma_uint32_4_2 res0.[0] res0.[2];
+
+  vec_interleave_low_n_lemma_uint32_4_2 res0.[1] res0.[3];
+  vec_interleave_high_n_lemma_uint32_4_2 res0.[1] res0.[3];
+
+  vec_interleave_low_lemma_uint32_4 vs.[0] vs.[1];
+  vec_interleave_high_lemma_uint32_4 vs.[0] vs.[1];
+
+  vec_interleave_low_lemma_uint32_4 vs.[2] vs.[3];
+  vec_interleave_high_lemma_uint32_4 vs.[2] vs.[3]
+
 
 val transpose8x8_lemma_ij: vs:lseq (uint32xN 8) 8 -> i:nat{i < 8} -> j:nat{j < 8} ->
   Lemma ((vec_v (transpose8x8 vs).[i]).[j] == (vec_v vs.[j]).[i])
 let transpose8x8_lemma_ij vs i j =
-  admit()
+  let res = transposewxw 3 vs in
+  Loop.unfold_repeati 3 (transposewxw_f 3) vs 2;
+  Loop.unfold_repeati 3 (transposewxw_f 3) vs 1;
+  Loop.unfold_repeati 3 (transposewxw_f 3) vs 0;
+  Loop.eq_repeati0 3 (transposewxw_f 3) vs;
+
+  let res0 = transposewxw_f 3 0 vs in
+  let res1 = transposewxw_f 3 1 res0 in
+  let res2 = transposewxw_f 3 2 res1 in
+
+  Classical.forall_intro (transposewxw_f_lemma_l #8 3 2 res1);
+  Classical.forall_intro (transposewxw_f_lemma_l #8 3 1 res0);
+  Classical.forall_intro (transposewxw_f_lemma_l #8 3 0 vs);
+
+  vec_interleave_low_n_lemma_uint32_8_4 res1.[0] res1.[4];
+  vec_interleave_low_n_lemma_uint32_8_4 res1.[1] res1.[5];
+  vec_interleave_low_n_lemma_uint32_8_4 res1.[2] res1.[6];
+  vec_interleave_low_n_lemma_uint32_8_4 res1.[3] res1.[7];
+  vec_interleave_high_n_lemma_uint32_8_4 res1.[0] res1.[4];
+  vec_interleave_high_n_lemma_uint32_8_4 res1.[1] res1.[5];
+  vec_interleave_high_n_lemma_uint32_8_4 res1.[2] res1.[6];
+  vec_interleave_high_n_lemma_uint32_8_4 res1.[3] res1.[7];
+
+  vec_interleave_low_n_lemma_uint32_8_2 res0.[0] res0.[2];
+  vec_interleave_low_n_lemma_uint32_8_2 res0.[1] res0.[3];
+  vec_interleave_low_n_lemma_uint32_8_2 res0.[4] res0.[6];
+  vec_interleave_low_n_lemma_uint32_8_2 res0.[5] res0.[7];
+  vec_interleave_high_n_lemma_uint32_8_2 res0.[0] res0.[2];
+  vec_interleave_high_n_lemma_uint32_8_2 res0.[1] res0.[3];
+  vec_interleave_high_n_lemma_uint32_8_2 res0.[4] res0.[6];
+  vec_interleave_high_n_lemma_uint32_8_2 res0.[5] res0.[7];
+
+  vec_interleave_low_lemma_uint32_8 vs.[0] vs.[1];
+  vec_interleave_low_lemma_uint32_8 vs.[2] vs.[3];
+  vec_interleave_low_lemma_uint32_8 vs.[4] vs.[5];
+  vec_interleave_low_lemma_uint32_8 vs.[6] vs.[7];
+  vec_interleave_high_lemma_uint32_8 vs.[0] vs.[1];
+  vec_interleave_high_lemma_uint32_8 vs.[2] vs.[3];
+  vec_interleave_high_lemma_uint32_8 vs.[4] vs.[5];
+  vec_interleave_high_lemma_uint32_8 vs.[6] vs.[7]
+
+
+#set-options "--z3rlimit 300"
 
 val transpose16x16_lemma_ij: vs:lseq (uint32xN 16) 16 -> i:nat{i < 16} -> j:nat{j < 16} ->
   Lemma ((vec_v (transpose16x16 vs).[i]).[j] == (vec_v vs.[j]).[i])
 let transpose16x16_lemma_ij vs i j =
-  admit()
+  let res = transposewxw 4 vs in
+  Loop.unfold_repeati 4 (transposewxw_f 4) vs 3;
+  Loop.unfold_repeati 4 (transposewxw_f 4) vs 2;
+  Loop.unfold_repeati 4 (transposewxw_f 4) vs 1;
+  Loop.unfold_repeati 4 (transposewxw_f 4) vs 0;
+  Loop.eq_repeati0 4 (transposewxw_f 4) vs;
+
+  let res0 = transposewxw_f 4 0 vs in
+  let res1 = transposewxw_f 4 1 res0 in
+  let res2 = transposewxw_f 4 2 res1 in
+  let res3 = transposewxw_f 4 3 res2 in
+
+  Classical.forall_intro (transposewxw_f_lemma_l #16 4 3 res2);
+  Classical.forall_intro (transposewxw_f_lemma_l #16 4 2 res1);
+  Classical.forall_intro (transposewxw_f_lemma_l #16 4 1 res0);
+  Classical.forall_intro (transposewxw_f_lemma_l #16 4 0 vs);
+
+  vec_interleave_low_n_lemma_uint32_16_8 res2.[0] res2.[8];
+  vec_interleave_low_n_lemma_uint32_16_8 res2.[1] res2.[9];
+  vec_interleave_low_n_lemma_uint32_16_8 res2.[2] res2.[10];
+  vec_interleave_low_n_lemma_uint32_16_8 res2.[3] res2.[11];
+  vec_interleave_low_n_lemma_uint32_16_8 res2.[4] res2.[12];
+  vec_interleave_low_n_lemma_uint32_16_8 res2.[5] res2.[13];
+  vec_interleave_low_n_lemma_uint32_16_8 res2.[6] res2.[14];
+  vec_interleave_low_n_lemma_uint32_16_8 res2.[7] res2.[15];
+
+  vec_interleave_high_n_lemma_uint32_16_8 res2.[0] res2.[8];
+  vec_interleave_high_n_lemma_uint32_16_8 res2.[1] res2.[9];
+  vec_interleave_high_n_lemma_uint32_16_8 res2.[2] res2.[10];
+  vec_interleave_high_n_lemma_uint32_16_8 res2.[3] res2.[11];
+  vec_interleave_high_n_lemma_uint32_16_8 res2.[4] res2.[12];
+  vec_interleave_high_n_lemma_uint32_16_8 res2.[5] res2.[13];
+  vec_interleave_high_n_lemma_uint32_16_8 res2.[6] res2.[14];
+  vec_interleave_high_n_lemma_uint32_16_8 res2.[7] res2.[15];
+
+  vec_interleave_low_n_lemma_uint32_16_4 res1.[0] res1.[4];
+  vec_interleave_low_n_lemma_uint32_16_4 res1.[1] res1.[5];
+  vec_interleave_low_n_lemma_uint32_16_4 res1.[2] res1.[6];
+  vec_interleave_low_n_lemma_uint32_16_4 res1.[3] res1.[7];
+  vec_interleave_low_n_lemma_uint32_16_4 res1.[8] res1.[12];
+  vec_interleave_low_n_lemma_uint32_16_4 res1.[9] res1.[13];
+  vec_interleave_low_n_lemma_uint32_16_4 res1.[10] res1.[14];
+  vec_interleave_low_n_lemma_uint32_16_4 res1.[11] res1.[15];
+
+  vec_interleave_high_n_lemma_uint32_16_4 res1.[0] res1.[4];
+  vec_interleave_high_n_lemma_uint32_16_4 res1.[1] res1.[5];
+  vec_interleave_high_n_lemma_uint32_16_4 res1.[2] res1.[6];
+  vec_interleave_high_n_lemma_uint32_16_4 res1.[3] res1.[7];
+  vec_interleave_high_n_lemma_uint32_16_4 res1.[8] res1.[12];
+  vec_interleave_high_n_lemma_uint32_16_4 res1.[9] res1.[13];
+  vec_interleave_high_n_lemma_uint32_16_4 res1.[10] res1.[14];
+  vec_interleave_high_n_lemma_uint32_16_4 res1.[11] res1.[15];
+
+  vec_interleave_low_n_lemma_uint32_16_2 res0.[0] res0.[2];
+  vec_interleave_low_n_lemma_uint32_16_2 res0.[1] res0.[3];
+  vec_interleave_low_n_lemma_uint32_16_2 res0.[4] res0.[6];
+  vec_interleave_low_n_lemma_uint32_16_2 res0.[5] res0.[7];
+  vec_interleave_low_n_lemma_uint32_16_2 res0.[8] res0.[10];
+  vec_interleave_low_n_lemma_uint32_16_2 res0.[9] res0.[11];
+  vec_interleave_low_n_lemma_uint32_16_2 res0.[12] res0.[14];
+  vec_interleave_low_n_lemma_uint32_16_2 res0.[13] res0.[15];
+
+  vec_interleave_high_n_lemma_uint32_16_2 res0.[0] res0.[2];
+  vec_interleave_high_n_lemma_uint32_16_2 res0.[1] res0.[3];
+  vec_interleave_high_n_lemma_uint32_16_2 res0.[4] res0.[6];
+  vec_interleave_high_n_lemma_uint32_16_2 res0.[5] res0.[7];
+  vec_interleave_high_n_lemma_uint32_16_2 res0.[8] res0.[10];
+  vec_interleave_high_n_lemma_uint32_16_2 res0.[9] res0.[11];
+  vec_interleave_high_n_lemma_uint32_16_2 res0.[12] res0.[14];
+  vec_interleave_high_n_lemma_uint32_16_2 res0.[13] res0.[15];
+
+  vec_interleave_low_lemma_uint32_16 vs.[0] vs.[1];
+  vec_interleave_low_lemma_uint32_16 vs.[2] vs.[3];
+  vec_interleave_low_lemma_uint32_16 vs.[4] vs.[5];
+  vec_interleave_low_lemma_uint32_16 vs.[6] vs.[7];
+  vec_interleave_low_lemma_uint32_16 vs.[8] vs.[9];
+  vec_interleave_low_lemma_uint32_16 vs.[10] vs.[11];
+  vec_interleave_low_lemma_uint32_16 vs.[12] vs.[13];
+  vec_interleave_low_lemma_uint32_16 vs.[14] vs.[15];
+
+  vec_interleave_high_lemma_uint32_16 vs.[0] vs.[1];
+  vec_interleave_high_lemma_uint32_16 vs.[2] vs.[3];
+  vec_interleave_high_lemma_uint32_16 vs.[4] vs.[5];
+  vec_interleave_high_lemma_uint32_16 vs.[6] vs.[7];
+  vec_interleave_high_lemma_uint32_16 vs.[8] vs.[9];
+  vec_interleave_high_lemma_uint32_16 vs.[10] vs.[11];
+  vec_interleave_high_lemma_uint32_16 vs.[12] vs.[13];
+  vec_interleave_high_lemma_uint32_16 vs.[14] vs.[15]
 
 
+#set-options "--z3rlimit 50"
 
 val transpose4x4_lemma: vs:lseq (uint32xN 4) 4 ->
   Lemma ((forall (i:nat{i < 4}) (j:nat{j < 4}). (vec_v (transpose4x4 vs).[i]).[j] == (vec_v vs.[j]).[i]))
